Conversion to and from DBV form

lambda-v-cs/Alpha.v
@@ -1,3 +1,4 @@
+Require Import List. 
 Require Import LambdaSyntax.
 Require Import DBVar. 
 
@@ -55,3 +56,89 @@ Proof.
   intros A t1 t2 Heq. rewrite Heq. apply alpha_equiv_refl. 
 Qed. 
 
+(** Equivalence of terms converted to and from a DeBruijn variation. *)
+
+Fixpoint well_formed_aux {A : Type} (dt : dbv_term A) (b : nat) : bool := 
+  match dt with
+    | DBV_const _ => true
+    | DBV_var (Free _) => true
+    | DBV_var (Bound n) => leb (S n) b
+    | DBV_abs body => well_formed_aux body (S b)
+    | DBV_app m n => andb (well_formed_aux m b) (well_formed_aux n b)
+  end. 
+
+Lemma well_formed_var : forall (A : Type) (v n : nat),
+                          well_formed_aux (DBV_var A (Bound v)) n = true -> 
+                          v < n.
+Proof. 
+  intros A v n H. 
+  simpl in H. destruct n. inversion H. apply le_lt_n_Sm. apply leb_complete. assumption. 
+Qed. 
+
+Lemma well_formed_higher : forall (A : Type) (dt : dbv_term A) (n : nat),
+                             well_formed_aux dt n = true -> well_formed_aux dt (S n) = true. 
+Proof. 
+  intros A dt. induction dt. 
+  (* Case dt = DBV_const *) reflexivity. 
+
+  (* Case dt = DBV_var *) 
+  intros n H. simpl. destruct d. reflexivity. 
+  apply well_formed_var in H. apply leb_correct. apply lt_le_weak; assumption. 
+
+  (* Case dt = DBV_abs *)
+  intros n H. 
+  simpl. simpl in H. apply IHdt. assumption. 
+
+  (* Case dt = DBV_app *)
+  intros n H. simpl in H. simpl. apply andb_prop in H. 
+  apply andb_true_intro. split; [ apply IHdt1 | apply IHdt2 ]; tauto. 
+Qed. 
+  
+(* 
+Lemma convert_well_formed_higher : 
+  forall (A : Type) (t : term A) v ls n,
+    well_formed_aux (convert_to_dbv_aux t ls) n = true -> 
+    well_formed_aux (convert_to_dbv_aux t (v::ls)) (S n) = true. 
+Proof. 
+  intros A t v ls n H. 
+  induction t. simpl. 
+
+
+Lemma convert_well_formed : forall (A : Type) (t : term A),
+                              well_formed_aux (convert_to_dbv t) 0 = true.
+Proof. 
+  intros A t. 
+  induction t. 
+  reflexivity. reflexivity. 
+  simpl. apply well_formed_higher. 
+*)
+
+Lemma to_from_dbv_eq : forall (A : Type) (dt : dbv_term A),
+                         well_formed_aux dt 0 = true -> 
+                         convert_to_dbv (dbv_to_term dt) = dt.
+Proof. 
+  intros A dt H. unfold dbv_to_term. unfold convert_to_dbv. induction dt. 
+  (* Case dt = DBV_const a *) reflexivity. 
+  
+  (* Case dt = DBV_var *) 
+  simpl. destruct d. reflexivity. 
+  assert (Hcontra: well_formed_aux ([| n # A |]) 0 = false). 
+  reflexivity. congruence. 
+
+  (* Case dt = DBV_abs dt *)
+  simpl. f_equal.
+
+  (* Case dt = dt1 $$ dt2 *)
+  simpl. 
+
+Theorem from_to_dbv_equiv : forall (A : Type) (t : term A),
+                              dbv_to_term (convert_to_dbv t) == t.
+Proof. 
+  intros A t. induction t. 
+
+  (* Case t = Var v *) reflexivity. 
+
+  (* Case t = Const a *) reflexivity. 
+
+  (* Case t = Abs v t *) unfold alpha_equiv. 
+  unfold convert_to_dbv. simpl. 
